code/chacha20poly1305/Hacl.Impl.Chacha20Poly1305.PolyCore.fsti
@@ -28,15 +28,15 @@ val poly1305_padded:
       modifies (loc tmp |+| loc ctx) h0 h1 /\
       Poly.state_inv_t h1 ctx /\
       // Additional framing for r_elem
-      Seq.index (Poly.as_get_r h0 ctx) 0 == Seq.index (Poly.as_get_r h1 ctx) 0 /\
+      Poly.as_get_r h0 ctx == Poly.as_get_r h1 ctx /\
       // Functional spec
-      Seq.index (Poly.as_get_acc h1 ctx) 0 == 
+      Poly.as_get_acc h1 ctx == 
       Spec.poly1305_padded 
-        (Seq.index (Poly.as_get_r h0 ctx) 0)
+        (Poly.as_get_r h0 ctx)
         (v len)
         (as_seq h0 text)
         (as_seq h0 tmp)
-        (Seq.index (Poly.as_get_acc h0 ctx) 0)
+        (Poly.as_get_acc h0 ctx)
         )
 
 val poly1305_init:
@@ -47,8 +47,8 @@ val poly1305_init:
     (ensures fun h0 _ h1 -> modifies (loc ctx) h0 h1 /\
       Poly.state_inv_t h1 ctx /\
       (let acc, r = SpecPoly.poly1305_init (as_seq h0 k) in
-      acc == Seq.index (Poly.as_get_acc h1 ctx) 0 /\
-      r == Seq.index (Poly.as_get_r h1 ctx) 0))
+      acc == Poly.as_get_acc h1 ctx /\
+      r == Poly.as_get_r h1 ctx))
 
 val update1:
   ctx:Poly.poly1305_ctx M32 ->
@@ -61,14 +61,14 @@ val update1:
       modifies (loc ctx) h0 h1 /\
       Poly.state_inv_t h1 ctx /\
       // Additional framing for r_elem
-      Seq.index (Poly.as_get_r h0 ctx) 0 == Seq.index (Poly.as_get_r h1 ctx) 0 /\    
+      Poly.as_get_r h0 ctx == Poly.as_get_r h1 ctx /\    
       // Functional spec
-      Seq.index (Poly.as_get_acc h1 ctx) 0 == 
+      Poly.as_get_acc h1 ctx == 
       SpecPoly.update1
-        (Seq.index (Poly.as_get_r h0 ctx) 0)
+        (Poly.as_get_r h0 ctx)
         (v len)
         (as_seq h0 text)
-        (Seq.index (Poly.as_get_acc h0 ctx) 0)
+        (Poly.as_get_acc h0 ctx)
         )
 
 val finish:
@@ -80,4 +80,4 @@ val finish:
       disjoint out k /\ disjoint out ctx /\ disjoint k ctx /\
       Poly.state_inv_t h ctx)
     (ensures fun h0 _ h1 -> modifies (loc out |+| loc ctx) h0 h1 /\
-      as_seq h1 out == SpecPoly.finish (as_seq h0 k) (Seq.index (Poly.as_get_acc h0 ctx) 0))
+      as_seq h1 out == SpecPoly.finish (as_seq h0 k) (Poly.as_get_acc h0 ctx))
